\documentclass[12pt]{article}

\usepackage[margin=0.6in]{geometry}
\setlength{\parindent}{0em}
\usepackage{mathtools}
\usepackage{amsmath}
\usepackage{collectbox}
\usepackage{array}
\usepackage{calc}

\begin{document}
\title{B503 Homework Assignment 2}
\author{Oyedotun Oyesanmi}
\date{\today}
\maketitle



\textbf{Answer 1:}
\begin{table}[h]
	\begin{center}
		\begin{tabular}{| >{\centering\arraybackslash}m{2in} | >{\centering\arraybackslash}m{1.5in} | >{\centering\arraybackslash}m{1in} | >{\centering\arraybackslash}m{1.5in} | >{\centering\arraybackslash}m{1.7in} |}
			\hline
			\textbf{Recurrence Relation} & \textbf{Linear} & \textbf{Non-zero coefficient} & \textbf{Non-homogeneous term}  \parbox{0pt}{\rule{0pt}{2ex+\baselineskip}}\\ \hline
			$A_n = 2A_{n-1} + 2^n$ & Yes & 2 & $2^n$ \parbox{0pt}{\rule{0pt}{3ex+\baselineskip}}\\  \hline
			\textbf{$A_n = log(n)A_{n-2} + 3A_{n-3}$} & Yes &  3 & None\parbox{0pt}{\rule{0pt}{3ex+\baselineskip}}\\  \hline
			\textbf{$A_n = A_{n-1}/A_{n-2} + 1$} & No & 1 & 1 \parbox{0pt}{\rule{0pt}{3ex+\baselineskip}}\\  \hline
		\end{tabular}
	\end{center}
\end{table}


\textbf{Answer 2:}\\
$$F_n = 6F_{n-1} - 9F_{n-2} $$

$C_1 = 6$ and $C_2 = -9$\\

We try to find the roots $r_1$ and $r_2$ of the characteristic equation $x^2 - C_1x - C_2 = 0$
\begin{align*}
&x^2 - (6)x - (-9) = 0\\
&x^2 + 6x + 9 = 0\\
\end{align*}
using factorization method
\begin{align*}
&x^2 - 3x - 3x - 9 = 0\\
&x(x-3) -3(x-3) = 0\\
&(x-3)(x-3) = 0\\
&x=3~or~ x=3\\
\end{align*}

roots of the equation are same i.e. $r_1 = r_2 = 3$\\

General solution for any given recurrence relation when $r_1 = r_2$ is\\

$$F_n = \alpha_1(r_1)^n + \alpha_2n(r_1) \text{~~~ for all $n \geq 0$}$$\\

substituting for $r_1$, we get
\begin{align*}
&= \alpha_1(3)^n + \alpha_2n(3)^n\\[7pt]
&= (\alpha_1 + \alpha_2n)3^n\\
\end{align*}

Therefore, the recurrence relation $F_n = 6F_{n-1} - 9F_{n-2} $ has solution $F_n = (\alpha_1 + \alpha_2n)3^n $, where $\alpha_1$ and $\alpha_2$ are any constants.\\\\

\textbf{Answer 3a:}\\

$A_0 = -2;~A_n = 3A_{n-1} ~$ for all $n \geq 1$\\

This is a 1\textsuperscript{th} order recurrence relationship, where\\
\begin{align*}
F_n = a . C^n \text{~~~~~~ for all $n \geq 0$}
\end{align*}

$a = -2; c = 3$\\

So the solution to the recurrence relation is:
$$A_n = (-2)(3)^n $$



\textbf{Answer 3b:}\\

$B_0 = 1;~B_1 = 8;~B_n = B_{n-1} + 2B_{n-2}~$ for all $n \geq 2$\\

$C_1 = -1$ and $C_2 = 2$\\

We try to find roots $r_1$ and $r_2$ of the characteristic equation $x^2 - C_1x - C_2$

\begin{align*}
&x^2 - (-1)x - 2\\
&x^2 + x - 2\\
\end{align*}

using quadratic formula $$ \frac{-b \pm  \sqrt[]{b^2 - 4ac}}{2a}$$

\begin{align*}
& \frac{-(-1)\pm  \sqrt[]{{-1}^2 - 4(1)(-2)}}{2(1)}\\[7pt]
&\frac{1\pm  \sqrt[]{9}}{2}\\[7pt]
&\frac{1\pm 3}{2}\\[7pt]
&\frac{1 + 3}{2} ~~ and ~~ \frac{1 - 3}{2} 
\end{align*}

roots of the equation are $r_1 = 2$ and $r_2 = -1$

\begin{align}
&A_0 = \alpha_1 + \alpha_2 = 1\\[7pt]
&A_1 = \alpha_1r_1 + \alpha_2r_2 = 8
\end{align}

from (1) we have 
\begin{align}
\alpha_2 = 1 - \alpha_1
\end{align}

substituting eq(3) in eq(2) we have
\begin{align*}
&\alpha_1r_1 + (1 - \alpha_1)r_2 = 8\\[7pt]
&\alpha_1r_1 + r_2 - \alpha_1r_2 = 8\\[7pt]
&\alpha_1(r_1 - r_2)  = 8 -r_2\\[7pt]
&\alpha_1 = \frac{8- r_2}{r_1 - r_2}
\end{align*}

substituting for $r_1 = 2$ and $r_2 = -1$

\begin{align*}
&\alpha_1 = \frac{8- (-1)}{2 - (-1)}\\[7pt]
&\alpha_1 = 3\\[7pt]
&\alpha_2 = 1 - \alpha_1\\[7pt]
&\alpha_2 = 1 - 3\\[7pt]
&\alpha_2 = -2
\end{align*}
So the solution to the recurrence relation is:
$$B_n = 3(2)^n +(-2)(-1)^n$$

\end{document}